src/axiomatic/TsoSimLocal.v
@@ -382,19 +382,19 @@ Proof.
 Qed.
 
 Definition sim_local_coh_cl ex loc :=
-  (⦗ex.(Execution.label_is) (Label.is_accessing_cl loc)⦘ ⨾
-   Execution.po).
+  ⦗ex.(Execution.label_is) (Label.is_kinda_writing_cl loc)⦘ ⨾
+  (Execution.rfe ex)^? ⨾
+  Execution.po.
 
 Lemma sim_local_coh_cl_step ex loc:
   sim_local_coh_cl ex loc =
   (sim_local_coh_cl ex loc ∪
-   (⦗ex.(Execution.label_is) (Label.is_accessing_cl loc)⦘)) ⨾
+   ⦗ex.(Execution.label_is) (Label.is_kinda_writing_cl loc)⦘ ⨾ (Execution.rfe ex)^?) ⨾
   Execution.po_adj.
 Proof.
-  unfold sim_local_coh_cl. rewrite ? (union_seq' Execution.po_adj), ? seq_assoc, ? union_assoc.
-  rewrite Execution.po_po_adj at 1.
+  unfold sim_local_coh_cl. rewrite Execution.po_po_adj at 1.
   rewrite (clos_refl_union Execution.po), union_seq, eq_seq.
-  rewrite ? (seq_union' (Execution.po ⨾ Execution.po_adj) Execution.po_adj), ? seq_assoc, ? union_assoc.
+  rewrite ? seq_union, ? union_seq, ? seq_assoc.
   refl.
 Qed.
 
@@ -410,23 +410,6 @@ Proof.
   - i. inv H. obtac.
     econs. simtac. econs; eauto.
     destruct l; ss; eapply Loc.cl_trans; eauto; eapply Loc.cl_sym; ss.
-Qed.
-
-Definition sim_local_coh_cl2 ex loc :=
-  (⦗ex.(Execution.label_is) (Label.is_writing_cl loc)⦘ ⨾
-   Execution.po).
-
-Lemma sim_local_coh_cl2_step ex loc:
-  sim_local_coh_cl2 ex loc =
-  (sim_local_coh_cl2 ex loc ∪
-   (⦗ex.(Execution.label_is) (Label.is_writing_cl loc)⦘)) ⨾
-  Execution.po_adj.
-Proof.
-  unfold sim_local_coh_cl2. rewrite ? (union_seq' Execution.po_adj), ? seq_assoc, ? union_assoc.
-  rewrite Execution.po_po_adj at 1.
-  rewrite (clos_refl_union Execution.po), union_seq, eq_seq.
-  rewrite ? (seq_union' (Execution.po ⨾ Execution.po_adj) Execution.po_adj), ? seq_assoc, ? union_assoc.
-  refl.
 Qed.
 
 Definition sim_local_vpn ex :=
